ITree_Deadlock.thy
@@ -24,12 +24,6 @@ lemma retvals_deadlock [simp]: "\<^bold>R(deadlock) = {}"
 definition deadlock_free :: "('e, 'r) itree \<Rightarrow> bool" where
 "deadlock_free P = (\<forall> tr. \<not> P \<midarrow>tr\<leadsto> deadlock)"
 
-lemma pdom_empty_iff_dom_empty: "f = {\<mapsto>} \<longleftrightarrow> dom f = {}"
-  by (metis pdom_res_empty pdom_res_pdom pdom_zero)
-
-lemma empty_map_pfunD [dest!]: "{\<mapsto>} = map_pfun f F \<Longrightarrow> F = {\<mapsto>}"
-  by (metis pdom_empty_iff_dom_empty pdom_map_pfun)
-
 lemma deadlock_free_deadlock: "deadlock_free deadlock = False"
   by (simp add: deadlock_free_def deadlock_trace_to)
 
@@ -38,6 +32,22 @@ lemma deadlock_free_Ret: "deadlock_free (\<checkmark> x)"
 
 lemma deadlock_free_Sil: "deadlock_free (Sil P) = deadlock_free P"
   by (metis deadlock_free_def itree.disc(5) stable_deadlock trace_to_Sil trace_to_SilE)
+
+lemma deadlock_free_VisI:
+  assumes 
+    "dom(F) \<noteq> {}" "\<And> e. e \<in> dom(F) \<Longrightarrow> deadlock_free (F(e)\<^sub>p)"
+  shows "deadlock_free (Vis F)"
+  by (metis assms deadlock_def deadlock_free_def itree.inject(3) pdom_zero trace_to_VisE)
+
+lemma deadlock_free_VisE:
+  assumes "deadlock_free (Vis F)"
+    "\<lbrakk> dom(F) \<noteq> {}; \<And> e. e \<in> pdom(F) \<Longrightarrow> deadlock_free (F(e)\<^sub>p) \<rbrakk> \<Longrightarrow> thesis"
+  shows thesis
+  by (metis assms deadlock_def deadlock_free_deadlock deadlock_free_def pdom_empty_iff_dom_empty trace_to.intros(3))
+
+lemma deadlock_free_Vis:
+  "deadlock_free (Vis F) = (dom(F) \<noteq> {} \<and> (\<forall>e\<in>pdom(F). deadlock_free (F(e)\<^sub>p)))"
+  by (auto intro: deadlock_free_VisI elim: deadlock_free_VisE)
 
 lemma deadlock_free_bindI: "\<lbrakk> deadlock_free P; \<forall> s\<in>\<^bold>R(P). deadlock_free (Q s) \<rbrakk> \<Longrightarrow> deadlock_free (P \<bind> Q)"
   apply (auto elim!:trace_to_bindE bind_VisE' simp add: deadlock_def deadlock_free_def)
